\documentclass[12pt]{article}
\pdfoutput=1
\usepackage{bm}% bold math
\usepackage{graphicx}
\graphicspath{}
%\usepackage{tabularx}
\usepackage{amsfonts}
\usepackage{amsmath}
\usepackage{amssymb}
\usepackage{amsbsy}
\usepackage{bbm}
\usepackage{hyperref}
\usepackage{mathdots}
\usepackage{booktabs}
\setlength{\heavyrulewidth}{1.5pt}
\setlength{\abovetopsep}{4pt}
\usepackage[margin=0.7in]{geometry}
\usepackage{nicefrac}
\usepackage{subcaption}
\newenvironment{psmallmatrix}
  {\left[\begin{matrix}}
  {\end{matrix}\right]}
  \usepackage{listings}


\begin{document}

\begin{center}
\begin{large}
GAUSSIAN-BINARY RESTRICTED BOLTZMANN MACHINES
\end{large}
\end{center}

\noindent Notation:
\begin{itemize}
\item visible nodes $\vec{x}  \in \mathbb{R}^M$ - gaussian units (position coordinates)
\item hidden nodes $\vec{h} \in \mathbb{R}^N$ - binary units
\item visible biases $\vec{a} \in \mathbb{R}^M$
\item hidden biases $\vec{b} \in \mathbb{R}^N$
\item interaction weights $\hat{W} \in \mathbb{R}^{M\times N}$
\item $j$th column vector of weight matrix $\vec{W}_j \in \mathbb{R}^M$
\item $i$th row vector of weight matrix $\vec{W}_i^T \in \mathbb{R}^N$ 
\item variational parameters $\vec{\theta} = ( a_0, \cdots, a_{M-1},b_0,\cdots,b_{N-1}, W_{0,0},\cdots,W_{M-1,N-1} )$ \\
\end{itemize}

\noindent "Energy" of a configuration of nodes:
\begin{align*}
E_{\vec{\theta}}(\vec{x},\vec{h}) &= \frac{1}{2\sigma^2} \sum_{i=0}^{M-1}(x_i - a_i)^2 - \sum_{j=0}^{N-1} b_j h_j -
\frac{1}{\sigma^2} \sum_{i=0}^{M-1}\sum_{j=0}^{N-1} x_i W_{ij} h_j\\
&= \frac{1}{2\sigma^2} \| \vec{x} - \vec{a} \|^2 - \vec{b}^T \vec{h} - \frac{1}{\sigma^2}\vec{x}^T \hat{W} \vec{h}
\end{align*}

\noindent Use the marginal probability to represent the wavefunction as a function of the RBM inputs:
\begin{align*}
\Psi_{\vec{\theta}}(\vec{x}) &= \frac{1}{Z} \sum_{\vec{h}} e^{-E_{\vec{\theta}}(\vec{x},\vec{h})}\\
&= \frac{1}{Z} \sum_{ \{ h_j \} } \exp \left( -\frac{1}{2\sigma^2} \sum_{i=0}^{M-1}(x_i - a_i)^2 + \sum_{j=0}^{N-1} b_j h_j + \frac{1}{\sigma^2} \sum_{i=0}^{M-1}\sum_{j=0}^{N-1} x_i W_{ij} h_j  \right)\\
&=\frac{1}{Z} \exp \left( -\frac{1}{2\sigma^2} \sum_{i=0}^{M-1}(x_i - a_i)^2 \right) \sum_{ \{ h_j \} } \exp \left( \sum_{j=0}^{N-1} b_j h_j + \frac{1}{\sigma^2} \sum_{i=0}^{M-1}\sum_{j=0}^{N-1} x_i W_{ij} h_j  \right)\\
&=\frac{1}{Z} \exp \left( -\frac{1}{2\sigma^2} \sum_{i=0}^{M-1}(x_i - a_i)^2 \right) \prod_{j=0}^{N-1} \sum_{ h_j=0 }^1 \exp \left( b_j h_j + \frac{1}{\sigma^2} \sum_{i=0}^{M-1} x_i W_{ij} h_j  \right)\\
&=\frac{1}{Z} \exp \left( -\frac{1}{2\sigma^2} \sum_{i=0}^{M-1}(x_i - a_i)^2 \right) \prod_{j=0}^{N-1} \left( 1 + \exp \left( b_j + \frac{1}{\sigma^2} \sum_{i=0}^{M-1} x_i W_{ij} \right) \right)\\
&= \frac{1}{Z} \exp \left( -\frac{1}{2\sigma^2} \| \vec{x}-\vec{a} \|^2 \right) \prod_{j=0}^{N-1} \left( 1 + \exp \left( b_j + \frac{1}{\sigma^2} \vec{x}^T \vec{W}_j \right) \right)
\end{align*}

\noindent Hamiltonian for $P$ $D$-dimensional particles in a harmonic oscillator:
\begin{align*}
\hat{H} = \frac{1}{2} \sum_{p = 0}^{P-1} \left( -\nabla_p^2 + \sum_{d=0}^{D-1} \omega_d^2 r_{p,d}^2 \right) + \sum_{p<q} V_{int} (r_{pq}), \ \ r_{pq} = \sqrt{ \sum_{d=0}^{D-1} (r_{p,d}-r_{q,d})^2 } 
\end{align*}




\noindent We need to vectorize the coordinates of all the particles to input into the RBM:
\begin{align*}
\vec{x} = ( r_{0,0}, \cdots, r_{0,D-1}, \cdots, r_{P-1,0}, \cdots, r_{P-1,D-1} ) \in \mathbb{R}^M, \ M = PD
\end{align*}
\noindent The visible biases and the rows of the weight matrix are organized in the same way. The mapping between coordinates and the visible nodes are:
\begin{align*}
r_{p,d} &= x_{Dp+d}\\
x_i &= r_{\text{floor}(i/D), i \text{mod} D}
\end{align*}

\noindent Now we can write our representation of the wavefunction as a function of all coordinates:
\begin{align*}
\Psi_{\vec{\theta}}(\vec{R}) &=\frac{1}{Z} \exp \left( -\frac{1}{2\sigma^2} \sum_{p=0}^{P-1}\sum_{d=0}^{D-1} (r_{p,d} - a_{Dp+d})^2 \right) \prod_{j=0}^{N-1} \left( 1 + \exp \left( b_j + \frac{1}{ \sigma^2} \sum_{p=0}^{P-1}\sum_{d=0}^{D-1} r_{p,d} W_{Dp+d,j} \right) \right)\\
&=\frac{1}{Z} \exp (A(\vec{R})) \prod_{j=0}^{N-1} \exp\left( \ln \left(  1 + \exp \left( b_j + \frac{1}{ \sigma^2} \sum_{p=0}^{P-1}\sum_{d=0}^{D-1} r_{p,d} W_{Dp+d,j} \right) \right) \right) \\
&=\frac{1}{Z} \exp (A(\vec{R})) \exp \left( \sum_{j=0}^{N-1} \ln \left(  1 + \exp \left( b_j + \frac{1}{ \sigma^2} \sum_{p=0}^{P-1}\sum_{d=0}^{D-1} r_{p,d} W_{Dp+d,j} \right) \right) \right) \\
&= \frac{1}{Z} \exp  \Big( A(\vec{R})+ B(\vec{R}) \Big) \\ \\
A(\vec{R}) &\equiv -\frac{1}{2\sigma^2} \sum_{p=0}^{P-1}\sum_{d=0}^{D-1} (r_{p,d} - a_{Dp+d})^2 = - \frac{1}{2\sigma^2}\sum_{i=0}^{M-1} (x_i-a_i)^2 = -\frac{1}{2\sigma^2} \| \vec{x} - \vec{a} \|^2\\
B(\vec{R}) &\equiv \sum_{j=0}^{N-1} \ln \left(  1 + \exp \left( B_j (\vec{R}) \right) \right)\\
B_j(\vec{R}) &\equiv b_j + \frac{1}{ \sigma^2}\sum_{p=0}^{P-1}\sum_{d=0}^{D-1} r_{p,d} W_{Dp+d,j} = b_j + \sum_{i=0}^{M-1} x_i W_{i,j} = b_j + \frac{1}{ \sigma^2} \vec{x}\cdot \vec{W}_j
\end{align*}

\noindent If the particles are bosons with a hard-core interaction:
\begin{align*}
V_{int} (r_{pq}) = 
\begin{cases} 
	\infty, & r_{pq} \leq a,\\
	0, & r_{pq} > a,
   \end{cases}
\end{align*}
and if the particles are electrons (fermions) with a repulsive Coulomb interaction ($e=1$):
\begin{align*}
V_{int} (r_{pq}) = \frac{1}{r_{pq}}
\end{align*}

\noindent The behaviors due to these interactions are accounted for in the trial wavefunction by a corresponding Jastrow factor so that the full trial wavefunction is 
\begin{align*}
\Psi (\vec{R}) = \frac{1}{Z} \exp \Big( A(\vec{R})+B(\vec{R})+J(\vec{R}) \Big)
\end{align*}
For bosons with a hard-core interaction:
\begin{align*}
J(\vec{R}) = \sum_{p<q} \ln \left( 1-\frac{a}{r_{pq}} \right)
\end{align*}
For electrons with the Coulomb interaction:
\begin{align*}
J(\vec{R}) = \sum_{p<q} \left( \frac{\alpha r_{pq}}{1+\beta r_{pq}} \right),
\end{align*}
where $\beta$ is a variational parameter and $\alpha$ is 1 when the electrons are anti-parallel and $\frac{1}{3}$ when the electrons are parallel.\\ \\

\noindent The local energy is defined as
\begin{align*}
E_L = \frac{1}{\Psi} \hat{H} \Psi
\end{align*}

\noindent We want an analytical expression for the local energy in terms of our variational parameters $\vec{\theta}$. First, we need the following quantities:

\begin{align*}
\nabla_k \{ \Psi \} &= \frac{1}{Z} \nabla_k \Big\{ \exp(A+B+J) \Big\} \\
&= \frac{1}{Z} \exp(A+B+J) \Big( \nabla_k \{ A \} + \nabla_k \{ B \} +\nabla_k \{ J \} \Big)\\
& = \Psi \Big( \nabla_k \{ A \} + \nabla_k \{ B \} +\nabla_k \{ J \} \Big) \\ \\
\nabla_k^2 \{\Psi \} &= \nabla_k \Big\{ \Psi \Big( \nabla_k \{ A \} + \nabla_k \{ B \} +\nabla_k \{ J \} \Big) \Big\}\\
&= \Psi \Big( \nabla_k^2 \{ A \} + \nabla_k^2 \{ B \} +\nabla_k^2 \{ J \} \Big) + \nabla_k \{ \Psi \} \Big( \nabla_k \{ A \} + \nabla_k \{ B \} +\nabla_k \{ J \} \Big)\\
&= \Psi \left(  \nabla_k^2 \{ A \} + \nabla_k^2 \{ B \} +\nabla_k^2 \{ J \}  + \Big( \nabla_k \{ A \} + \nabla_k \{ B \} +\nabla_k \{ J \} \Big)^2 \right)\\ \\ 
\frac{1}{\Psi} \nabla_k^2 \{ \Psi \} &= \nabla_k^2 \{ A \} + \nabla_k^2 \{ B \} +\nabla_k^2 \{ J \}  + \Big( \nabla_k \{ A \} + \nabla_k \{ B \} +\nabla_k \{ J \} \Big)^2\\ \\
\end{align*}

\noindent Let $\hat{n_d}$, $d = 0, ..., D-1$, denote the elementary unit vectors in each of the $D$ dimensions. Then,

\begin{align*}
A(\vec{R}) &\equiv -\frac{1}{2\sigma^2} \sum_{p=0}^{P-1}\sum_{d=0}^{D-1} (r_{p,d} - a_{Dp+d})^2,\\
\nabla_k \{A\}
&= \sum_{d'=0}^{D-1} \frac{\partial A}{\partial r_{k,d'}} \hat{n_{d'}} = \sum_{d'=0}^{D-1} \frac{\partial}{\partial r_{k,d'}} \bigg\{ -\frac{1}{2\sigma^2} \sum_{p=0}^{P-1}\sum_{d=0}^{D-1} (r_{p,d} - a_{Dp+d})^2 \bigg\} \hat{n_{d'}} \\
&= \sum_{d'=0}^{D-1} \frac{\partial}{\partial r_{k,d'}} \bigg\{ -\frac{1}{2\sigma^2}  (r_{k,d'} - a_{Dk+d'})^2 \bigg\} \hat{n_{d'}} = \frac{1}{\sigma^2} \sum_{d=0}^{D-1} (a_{Dk+d} -r_{k,d} ) \hat{n_{d}}  \\
\nabla_k^2 \{A\} &= \nabla_k \cdot \nabla_k\{A\} = \nabla_k \cdot \frac{1}{\sigma^2} \sum_{d=0}^{D-1} (a_{Dk+d} -r_{k,d} ) \hat{n_{d}} = \frac{1}{\sigma^2} \sum_{d=0}^{D-1} (-1) = -\frac{D}{\sigma^2}\\ 
\end{align*}


\begin{align*}
B_j(\vec{R}) &\equiv b_j + \frac{1}{\sigma^2} \sum_{p=0}^{P-1}\sum_{d=0}^{D-1} r_{p,d} W_{Dp+d,j}\\
\nabla_k \{ B_j \}  &= \sum_{d'=0}^{D-1} \frac{\partial B_j}{\partial r_{k,d'}} \hat{n}_{d'} = \sum_{d'=0}^{D-1} \frac{\partial}{\partial r_{k,d'}} \bigg\{ b_j + \frac{1}{\sigma^2} \sum_{p=0}^{P-1}\sum_{d=0}^{D-1} r_{p,d} W_{Dp+d,j} \bigg\} \hat{n}_{d'}\\
&= \frac{1}{\sigma^2} \sum_{d'=0}^{D-1} \frac{\partial}{\partial r_{k,d'}} \left[ r_{k,d'} W_{Dk+d',j} \right] \hat{n}_{d'} = \frac{1}{\sigma^2} \sum_{d=0}^{D-1} W_{Dk+d,j} \hat{n}_d \\
\nabla_k^2 \{ B_j \} &= 0\\ \\
B(\vec{R}) &\equiv \sum_{j=0}^{N-1} \ln \left(  1 + \exp \left( B_j (\vec{R}) \right) \right)\\
\nabla_k \{ B \} &= \nabla_k \bigg\{ \sum_{j=0}^{N-1} \ln \left(  1 + \exp \left( B_j \right) \right) \bigg\}= \sum_{j=0}^{N-1}\nabla_k \bigg\{  \ln \left(  1 + \exp \left( B_j \right) \right) \bigg\} \\
&=\sum_{j=0}^{N-1} \frac{1}{1+\exp(B_j)} \nabla_k \Big\{ 1+\exp(B_j) \Big\} 
=\sum_{j=0}^{N-1} \frac{\exp(B_j)}{1+\exp(B_j)} \nabla_k \{ B_j \}\\
&=\sum_{j=0}^{N-1} \frac{\nabla_k \{ B_j \}}{\exp(-B_j)+1}  = \frac{1}{\sigma^2} \sum_{d=0}^{D-1} \sum_{j=0}^{N-1}  \frac{W_{Dk+d,j}}{\exp(-B_j)+1}   \hat{n}_d \\
\nabla_k^2 \{ B\} &= \nabla_k \cdot \nabla_k \{ B \} = \nabla_k \cdot \bigg\{  \sum_{j=0}^{N-1} \frac{\nabla_k \{ B_j \}}{\exp(-B_j)+1}  \bigg\}\\
&= \sum_{j=0}^{N-1} \left[ \nabla_k \Big\{ \frac{1}{\exp(-B_j)+1} \Big\} \cdot \nabla_k \{ B_j \} + \frac{\nabla_k^2 \{ B_j \}}{\exp(-B_j)+1} \right]\\
&= \sum_{j=0}^{N-1} \frac{\exp(-B_j)}{(\exp(-B_j)+1)^2} \nabla_k \{ B_j \} \cdot \nabla_k \{ B_j \}\\
&= \frac{1}{\sigma^4} \sum_{j=0}^{N-1} \frac{\exp(-B_j)}{(\exp(-B_j)+1)^2} \sum_{d=0}^{D-1} W_{Dk+d,j}^2
\end{align*}

\begin{align*}
r_{pq} &= \left( \sum_{d=0}^{D-1} (r_{p,d}-r_{q,d})^2 \right)^{1/2}\\
\nabla_k \{ r_{pq} \} &= \frac{1}{2} \left( \sum_{d=0}^{D-1} (r_{p,d}-r_{q,d})^2 \right)^{-1/2} \nabla_k \bigg\{ \sum_{d=0}^{D-1} (r_{p,d}-r_{q,d})^2 \bigg\} \\
&= \frac{1}{2 r_{pq}} \sum_{d=0}^{D-1} 2(r_{p,d}-r_{q,d})(\delta_{k,p}-\delta_{k,q}) \hat{n}_{d} = \frac{1}{r_{pq}} \sum_{d=0}^{D-1} (r_{p,d}-r_{q,d}) (\delta_{k,p}-\delta_{k,q}) \hat{n}_{d} \\ \\
J(\vec{R}) &= \sum_{p<q} \ln \left( 1-\frac{a}{r_{pq}} \right)\\
\nabla_k \{ J \} &= \sum_{p<q} \frac{1}{1-\frac{a}{r_{pq}}} \nabla_{k} \left( 1-\frac{a}{r_{pq}} \right) 
= \sum_{p<q} \frac{r_{pq}}{r_{pq}-a} \frac{a}{r_{pq}^2} \nabla_k \{ r_{pq} \}\\
&= \sum_{p<q} \frac{1}{r_{pq}-a} \frac{a}{r_{pq}} \frac{1}{r_{pq}} \sum_{d=0}^{D-1} (r_{p,d}-r_{q,d})(\delta_{k,p}-\delta_{k,q}) \hat{n}_{d}\\
&= \sum_{d=0}^{D-1} \frac{1}{2} \sum_{p\neq q} \frac{(r_{p,d}-r_{q,d})(\delta_{k,p}-\delta_{k,q})}{r_{pq}^2(\frac{r_{pq}}{a}-1)} \hat{n}_d\\
&= \sum_{d=0}^{D-1} \frac{1}{2} \left[ \sum_{q \neq k} \frac{r_{k,d}-r_{q,d}}{r_{kq}^2 \left( \frac{r_{kq}}{a} -1 \right)} - \sum_{k \neq k} \frac{r_{p,d}-r_{k,d}}{r_{pk}^2 \left( \frac{r_{pk}}{a} -1 \right)} \right]\hat{n}_d\\
&= \sum_{d=0}^{D-1} \frac{1}{2} \left[2 \sum_{p \neq k} \frac{r_{k,d}-r_{p,d}}{r_{kp}^2 \left( \frac{r_{kp}}{a} -1 \right)} \right]\hat{n}_d = \sum_{d=0}^{D-1} \sum_{p=0, \ p\neq k}^{P-1} \frac{r_{k,d}-r_{p,d}}{r_{kp}^2 \left( \frac{r_{kp}}{a} -1 \right)} \hat{n}_d\\ 
\nabla_k^2 \{ J \} &= \sum_{d'=0}^{D-1} \hat{n}_{d'} \frac{\partial}{\partial r_{k,d'}} \cdot \bigg\{ \sum_{d=0}^{D-1} \sum_{p=0, \ p\neq k}^{P-1} \frac{r_{k,d}-r_{p,d}}{r_{kp}^2 \left( \frac{r_{kp}}{a} -1 \right)} \hat{n}_d  \bigg\} \\
&= \sum_{d=0}^{D-1} \sum_{p=0, \ p\neq k}^{P-1} \frac{\partial}{\partial r_{k,d}} \bigg\{ \frac{r_{k,d}-r_{p,d}}{r_{kp}^2 \left( \frac{r_{kp}}{a} -1 \right)} \bigg\} \\
&= \sum_{d=0}^{D-1} \sum_{p=0, \ p\neq k}^{P-1} 
\left[ (r_{k,d}-r_{p,d})
\frac{\partial}{\partial r_{k,d}} \bigg\{ r_{kp}^{-2}\left( \frac{r_{kp}}{a} -1 \right)^{-1} \bigg\} + \frac{\partial}{\partial r_{k,d}} \Big\{ r_{k,d}-r_{p,d}  \Big\} \frac{1}{r_{kp}^2 \left( \frac{r_{kp}}{a} -1 \right)}
\right]\\
&= \sum_{d=0}^{D-1} \sum_{p=0, \ p\neq k}^{P-1} 
\left[ (r_{k,d}-r_{p,d})
\left[ r_{kp}^{-2} \frac{\partial}{\partial r_{k,d}} \bigg\{ \left( \frac{r_{kp}}{a} -1 \right)^{-1} \bigg\} + \frac{\partial}{\partial r_{k,d}} \Big\{ r_{kp}^{-2} \Big\} \left( \frac{r_{kp}}{a} -1 \right)^{-1} \right]
 + \frac{1}{r_{kp}^2 \left( \frac{r_{kp}}{a} -1 \right)}
\right]\\
&= \sum_{d=0}^{D-1} \sum_{p=0, \ p\neq k}^{P-1} 
\left[ (r_{k,d}-r_{p,d})
\left[ 
\frac{-1}{a r_{kp}^2} \left( \frac{r_{kp}}{a} -1 \right)^{-2}
 \frac{\partial}{\partial r_{k,d}} \Big\{ r_{kp} \Big\} 
+ \frac{-2}{r_{kp}^3}  \frac{\partial}{\partial r_{k,d}} \Big\{ r_{kp} \Big\} \left( \frac{r_{kp}}{a} -1 \right)^{-1} 
\right] \right. \\
& \hspace*{2.75cm}  \left.
 + \frac{1}{r_{kp}^2 \left( \frac{r_{kp}}{a} -1 \right)}
\right]\\
&= \sum_{d=0}^{D-1} \sum_{p=0, \ p\neq k}^{P-1} 
\left[ -\frac{(r_{k,d}-r_{p,d})}{r_{kp}^2} \left( \frac{r_{kp}}{a} -1 \right)^{-1}  \frac{\partial}{\partial r_{k,d}} \Big\{ r_{kp} \Big\}
\left[ 
\frac{1}{a} \left( \frac{r_{kp}}{a} -1 \right)^{-1} 
+ \frac{2}{r_{kp}}
\right] 
+ \frac{1}{r_{kp}^2 \left( \frac{r_{kp}}{a} -1 \right)}
\right]
\end{align*}
\begin{align*}
\nabla_k^2\{ J \} 
&= \sum_{d=0}^{D-1} \sum_{p=0, \ p\neq k}^{P-1} 
\left[ -\frac{(r_{k,d}-r_{p,d})}{r_{kp}^2 \left( \frac{r_{kp}}{a} -1 \right)}  \left( \frac{r_{k,d}-r_{p,d}}{r_{kp}} \right)
\left[ 
\frac{1}{r_{kp}-a}
+ \frac{2}{r_{kp}}
\right] 
+ \frac{1}{r_{kp}^2 \left( \frac{r_{kp}}{a} -1 \right)}
\right]\\
&= \sum_{d=0}^{D-1} \sum_{p=0, \ p\neq k}^{P-1}  \frac{1}{r_{kp}^2 \left( \frac{r_{kp}}{a} -1 \right)}
\left[ 
-\frac{(r_{k,d}-r_{p,d})^2}{r_{kp}} \left[ \frac{3r_{kp}-2a}{r_{kp}(r_{kp}-a)} \right] +1
\right]\\
&= \sum_{d=0}^{D-1} \sum_{p=0, \ p\neq k}^{P-1}  \frac{1}{r_{kp}^2 \left( \frac{r_{kp}}{a} -1 \right)}
\left[ 
\left( \frac{r_{k,d}-r_{p,d}}{r_{kp}} \right)^2 \frac{2a-3r_{kp}}{r_{kp}-a}
 +1
\right]\\
\end{align*}


Putting all this together...
\begin{align*}
E_L &= \frac{1}{\Psi} \left[ \frac{1}{2} \sum_{p=0}^{P-1} -\nabla_p^2 + \frac{1}{2}\sum_{d=0}^{D-1} \omega_d^2r_{p,d}^2 \right] \Psi \\
&= -\frac{1}{2} \sum_{k=0}^{P-1} \frac{1}{\Psi} \nabla_k^2 \Psi + \frac{1}{2} \sum_{p=0}^{P-1} \sum_{d=0}^{D-1} \omega_d^2r_{p,d}^2\\
&= -\frac{1}{2} \sum_{k=0}^{P-1} 
\bigg( \nabla_k^2 \{ A \}  + \nabla_k^2 \{ B \}  + \nabla_k^2 \{ J \} + \Big( \nabla_k \{ A \}  + \nabla_k \{ B \}  + \nabla_k \{ J \}\Big)^2 \bigg)
+ \frac{1}{2} \sum_{p=0}^{P-1} \sum_{d=0}^{D-1} \omega_d^2r_{p,d}^2\\
%%%%%%%%%%%%%%%%%%%%
&= -\frac{1}{2} \sum_{k=0}^{P-1} 
\Bigg( -\frac{D}{\sigma^2}  + \frac{1}{\sigma^4} \sum_{j=0}^{N-1} \frac{\exp(-B_j)}{(\exp(-B_j)+1)^2} \sum_{d=0}^{D-1} W_{Dk+d,j}^2  \\
& \hspace*{2.5 cm} 
+ \sum_{d=0}^{D-1} \sum_{p=0, \ p\neq k}^{P-1}  \frac{1}{r_{kp}^2 \left( \frac{r_{kp}}{a} -1 \right)}
\left[ 
\left( \frac{r_{k,d}-r_{p,d}}{r_{kp}} \right)^2 \frac{2a-3r_{kp}}{r_{kp}-a}
 +1
\right]\\
& \hspace*{2.5 cm}
 + \bigg( \frac{1}{\sigma^2} \sum_{d=0}^{D-1} (a_{Dk+d} -r_{k,d} ) \hat{n_{d}}  
 + \frac{1}{\sigma^2} \sum_{d=0}^{D-1} \sum_{j=0}^{N-1}  \frac{W_{Dk+d,j}}{\exp(-B_j)+1}   \hat{n}_d  
 + \sum_{d=0}^{D-1} \sum_{p=0, \ p\neq k}^{P-1} \frac{r_{k,d}-r_{p,d}}{r_{kp}^2 \left( \frac{r_{kp}}{a} -1 \right)} \hat{n}_d
 \bigg)^2 \Bigg)\\
& \hspace*{.5 cm} + \frac{1}{2} \sum_{p=0}^{P-1} \sum_{d=0}^{D-1} \omega_d^2r_{p,d}^2\\
%%%%%%%%%%%%%%%%%%%%
&= -\frac{1}{2} \sum_{k=0}^{P-1} 
\Bigg( \sum_{d=0}^{D-1} \bigg[ \frac{1}{\sigma^4} \sum_{j=0}^{N-1} \frac{\exp(-B_j)W_{Dk+d,j}^2}{(\exp(-B_j)+1)^2}
+ \sum_{p=0, \ p\neq k}^{P-1}  \frac{1}{r_{kp}^2 \big( \frac{r_{kp}}{a} -1 \big)}
\Big[ 
\Big( \frac{r_{k,d}-r_{p,d}}{r_{kp}} \Big)^2 \frac{2a-3r_{kp}}{r_{kp}-a}
 +1
\Big]  \bigg] \\
& \hspace*{2.25 cm}
+ \bigg( \sum_{d=0}^{D-1} \bigg[
\frac{1}{\sigma^2}(a_{Dk+d} -r_{k,d} )
+\frac{1}{\sigma^2}\sum_{j=0}^{N-1}  \frac{W_{Dk+d,j}}{\exp(-B_j)+1}
+\sum_{p=0, \ p\neq k}^{P-1} \frac{r_{k,d}-r_{p,d}}{r_{kp}^2 \left( \frac{r_{kp}}{a} -1 \right)}
 \bigg] \hat{n_{d}}
 \bigg)^2 \Bigg)\\
& \hspace*{.5 cm} + \frac{PD}{2\sigma^2}+ \frac{1}{2}\sum_{p=0}^{P-1} \sum_{d=0}^{D-1} \omega_d^2r_{p,d}^2\\
%%%%%%%%%%%%%%%%%%%%
&= -\frac{1}{2} \sum_{k=0}^{P-1} \sum_{d=0}^{D-1}
\Bigg[ \frac{1}{\sigma^4} \sum_{j=0}^{N-1} \frac{\exp(-B_j)W_{Dk+d,j}^2}{(\exp(-B_j)+1)^2}
+ \sum_{p=0, \ p\neq k}^{P-1}  \frac{1}{r_{kp}^2 \big( \frac{r_{kp}}{a} -1 \big)}
\Big[ 
\Big( \frac{r_{k,d}-r_{p,d}}{r_{kp}} \Big)^2 \frac{2a-3r_{kp}}{r_{kp}-a}
 +1
\Big]  \\
& \hspace*{2.25 cm}
+ \bigg( 
\frac{1}{\sigma^2}(a_{Dk+d} -r_{k,d} )
+\frac{1}{\sigma^2}\sum_{j=0}^{N-1}  \frac{W_{Dk+d,j}}{\exp(-B_j)+1}
+\sum_{p=0, \ p\neq k}^{P-1} \frac{r_{k,d}-r_{p,d}}{r_{kp}^2 \left( \frac{r_{kp}}{a} -1 \right)}
 \bigg)^2  \Bigg]\\
& \hspace*{.5 cm} + \frac{PD}{2\sigma^2}+\frac{1}{2} \sum_{p=0}^{P-1} \sum_{d=0}^{D-1} \omega_d^2r_{p,d}^2\\
\end{align*}

\noindent To write $E_L$ in terms of the inputs $x_i$, we define the distance between the $k$th and $p$th particle as
\begin{align*}
R_i(p) &\equiv r_{kp}= \left( \sum_{d=0}^{D-1} (r_{k,d}-r_{p,d})^2 \right)^{1/2}\\
 &= r_{(\text{floor}(i/D))p} 
 = \left( \sum_{d=0}^{D-1} (x_{D(\text{floor}(i/D))+d}-x_{Dp+d})^2 \right)^{1/2}\\
\end{align*}
\noindent Then,
\begin{align*}
E_L &= -\frac{1}{2} \sum_{i=0}^{M-1}
\Bigg[ \frac{1}{\sigma^4} \sum_{j=0}^{N-1} \frac{\exp(-B_j)W_{i,j}^2}{(\exp(-B_j)+1)^2}\\
& \hspace*{2.25 cm}
+ a \sum_{p=0, \ p\neq \text{floor}(i/D)}^{P-1}  \frac{1}{R_i(p)^2 \big( R_i(p)-a \big)}
\Big[ 
\Big( \frac{x_i-x_{Dp+(i\text{mod}D)}}{R_i(p)} \Big)^2 \frac{2a-3R_i(p)}{R_i(p)-a}
 +1
\Big]  \\
& \hspace*{2.25 cm}
+ \bigg( 
\frac{1}{\sigma^2} (a_i -x_i )
+\frac{1}{\sigma^2} \sum_{j=0}^{N-1}  \frac{W_{i,j}}{\exp(-B_j)+1}
+a\sum_{p=0, \ p\neq \text{floor}(i/D)}^{P-1} \frac{x_i-x_{Dp+(i\text{mod}D)}}{R_i(p)^2 \left( R_i(p) -a \right)}
 \bigg)^2  \Bigg]\\
& \hspace*{.5 cm} + \frac{M}{2\sigma^2}+ \frac{1}{2} \sum_{i=0}^{M-1} \omega_{i\text{mod}D}^2x_i^2\\ \\ 
%%%%%%%%%%%%%%%%%%%%%%%%%%%%%%%%%%%%%%%%%%%%%%
&=-\frac{1}{2\sigma^4} \sum_{j=0}^{N-1}\frac{\exp(-B_j)}{(\exp(-B_j)+1)^2} \sum_{i=0}^{M-1}W_{i,j}^2 \\
& \hspace*{.5 cm}
-\frac{a}{2} \sum_{i=0}^{M-1} \sum_{p=0, \ p\neq \text{floor}(i/D)}^{P-1}\frac{1}{R_i(p)^2 \big( R_i(p)-a \big)}\Big[ \Big( \frac{x_i-x_{Dp+(i\text{mod}D)}}{R_i(p)} \Big)^2 \frac{2a-3R_i(p)}{R_i(p)-a}+1\Big]  \\
& \hspace*{.5 cm}
-\frac{1}{2} \sum_{i=0}^{M-1} \bigg( 
\frac{1}{\sigma^2}(a_i -x_i )
+\frac{1}{\sigma^2} \sum_{j=0}^{N-1}  \frac{W_{i,j}}{\exp(-B_j)+1}
+a\sum_{p=0, \ p\neq \text{floor}(i/D)}^{P-1} \frac{x_i-x_{Dp+(i\text{mod}D)}}{R_i(p)^2 \left( R_i(p) -a \right)}
 \bigg)^2\\
 & \hspace*{.5 cm} + \frac{M}{2\sigma^2}+\frac{1}{2} \sum_{i=0}^{M-1} \omega_{i\text{mod}D}^2x_i^2\\ \\ 
 %%%%%%%%%%%%%%%%%%%%%%%%%%%%%%%%%%%%%%%%%%%%%%
&=-\frac{1}{2\sigma^4} \sum_{j=0}^{N-1}\frac{\exp(-B_j)}{(\exp(-B_j)+1)^2} \vec{W}_j \cdot \vec{W}_j \\
& \hspace*{.5 cm}
-\frac{a}{2} \sum_{i=0}^{M-1} \sum_{p=0, \ p\neq \text{floor}(i/D)}^{P-1}\frac{1}{R_i(p)^2 \big( R_i(p)-a \big)}\Big[ \Big( \frac{x_i-x_{Dp+(i\text{mod}D)}}{R_i(p)} \Big)^2 \frac{2a-3R_i(p)}{R_i(p)-a}+1\Big]  \\
& \hspace*{.5 cm}
-\frac{1}{2} \sum_{i=0}^{M-1} \bigg( 
\frac{1}{\sigma^2} (a_i -x_i )
+\frac{1}{\sigma^2} \sum_{j=0}^{N-1}  \frac{W_{i,j}}{\exp(-B_j)+1}
+a\sum_{p=0, \ p\neq \text{floor}(i/D)}^{P-1} \frac{x_i-x_{Dp+(i\text{mod}D)}}{R_i(p)^2 \left( R_i(p) -a \right)}
 \bigg)^2\\
 & \hspace*{.5 cm} + \frac{M}{2\sigma^2}+ \frac{1}{2}(\Omega\%\Omega)\cdot (\vec{x}\% \vec{x})\\ \\ 
\end{align*}

\noindent In the last line, we have defined a vector $\vec{\Omega}$ with elements $\Omega_i = \omega_{i\text{mod}D}$. To increase the computational speed, we will precalculate and store the values $B_j$ in a vector $\vec{B}$ and store the following factors in a vector $\vec{f} \in \mathbb{R}^{N}$:
\begin{align*}
f_j \equiv \frac{1}{\exp(-B_j)+1}
\end{align*}

\noindent Then, the local energy becomes
\begin{align*}
E_L &=-\frac{1}{2} \sum_{j=0}^{N-1}\exp(-B_j) \Big\| \frac{f_j\vec{W}_j}{\sigma^2} \Big\|^2 + \frac{M}{2\sigma^2}+ \frac{1}{2}(\Omega\%\Omega)\cdot (\vec{x}\% \vec{x})\\
& \hspace*{.5 cm}
-\frac{a}{2} \sum_{i=0}^{M-1} \sum_{p=0, \ p\neq \text{floor}(i/D)}^{P-1}\frac{1}{R_i(p)^2 \big( R_i(p)-a \big)}\Big[ \Big( \frac{x_i-x_{Dp+(i\text{mod}D)}}{R_i(p)} \Big)^2 \frac{2a-3R_i(p)}{R_i(p)-a}+1\Big]  \\
& \hspace*{.5 cm}
-\frac{1}{2} \sum_{i=0}^{M-1} \bigg( 
\frac{1}{\sigma^2}(a_i -x_i )
+\frac{1}{\sigma^2} \vec{W}_i^T\vec{f}
+a\sum_{p=0, \ p\neq \text{floor}(i/D)}^{P-1} \frac{x_i-x_{Dp+(i\text{mod}D)}}{R_i(p)^2 \left( R_i(p) -a \right)}
 \bigg)^2\\
\end{align*}

\noindent For stochastic gradient descent, we will also need the gradient of the local energy with respect to the RBM parameters $\vec{\theta}=(\vec{a},\vec{b},\hat{W})$:
\begin{align*}
G_k = \frac{\partial \langle E_L \rangle}{\partial \theta_k} = 2 \left( \left\langle E_L \frac{1}{\Psi} \frac{\partial \Psi}{\partial \theta_k} \right\rangle - \left\langle E_L \right\rangle \left\langle \frac{1}{\Psi} \frac{\partial \Psi}{\partial \theta_k} \right\rangle \right)\\
\end{align*}



\noindent The derivatives of our new wavefunction with respect to the variational parameters are given by:
\begin{align*}
\frac{\partial \Psi}{\partial \vec{a}} &= \Psi \frac{\partial A(\vec{a})}{\partial \vec{a}} = \Psi \frac{\vec{x}-\vec{a}}{\sigma^2}\\
\frac{\partial \Psi}{\partial \vec{b}} &= \Psi \frac{\partial B(\vec{b},\hat{W})}{\partial \vec{b}} = \Psi \vec{f} \\
\frac{\partial \Psi}{\partial \hat{W}} &= \Psi \frac{\partial B(\vec{b},\hat{W})}{\partial \hat{W}}
= \Psi \frac{\vec{x} \vec{f}^T}{\sigma^2}
\end{align*}


\noindent The quantum force on the $k$th particle is defined as 
\begin{align}
\vec{F}_k(\vec{R}) = 2 \frac{1}{\Psi} \nabla_k \Psi.
\end{align}

\noindent Using the derivatives we have already calculated, we have
\begin{align*}
\vec{F}_k(\vec{R}) &= 2 \Big( \nabla_k \{ A \} + \nabla_k \{ B \} +\nabla_k \{ J \} \Big)\\
&= 2 \bigg( \sum_{d=0}^{D-1} (a_{Dk+d} -r_{k,d} ) \hat{n_{d}}  
 + \sum_{d=0}^{D-1} \sum_{j=0}^{N-1}  \frac{W_{Dk+d,j}}{\exp(-B_j)+1}   \hat{n}_d  
 + \sum_{d=0}^{D-1} \sum_{p=0, \ p\neq k}^{P-1} \frac{r_{k,d}-r_{p,d}}{r_{kp}^2 \left( \frac{r_{kp}}{a} -1 \right)} \hat{n}_d
 \bigg)\\
 &= 2 \sum_{d=0}^{D-1} \bigg[  (a_{Dk+d} -r_{k,d} ) 
 + \vec{W}_{Dk+d}^T\vec{f}   
 +  a \sum_{p=0, \ p\neq k}^{P-1} \frac{r_{k,d}-r_{p,d}}{r_{kp}^2 \left( r_{kp}-a \right)} 
 \bigg]\hat{n}_d\\
\end{align*}

\noindent The Langevin and Fokker-Planck equations give a new position $y$ from the old position $x$:
\begin{align}
y = x + d\Delta tF(x) + \xi \sqrt{\Delta t},
\end{align}
where $d=0.5$ is the diffusion constant and $\Delta t \in [0.001,0.01]$ is a chosen time step. \\

The transition probability is given by the Green's function
\begin{align}
G(y,x)=\frac{1}{(4\pi d \Delta t)^{3N/2}} \exp \left( -\frac{(y-x-d\Delta t F(x))^2}{4 d \Delta t} \right),
\end{align}
so that the Metropolis-Hastings acceptance ratio is
\begin{align}
A(y,x) = \min \{ 1, P(y,x) \},
\end{align}
where 
\begin{align*}
P(y,x) &= \frac{G(x,y) | \Psi_T(y) | ^2}{G(y,x) | \Psi_T(x) | ^2}\\
&= \exp \left( -\frac{(x-y-d\Delta t F(y))^2}{4 d \Delta t} \right) \exp \left( \frac{(y-x-d\Delta t F(x))^2}{4 d \Delta t} \right) \frac{| \Psi_T(y) | ^2}{ | \Psi_T(x) | ^2}\\
&= \exp \left( -\frac{(x-y)^2-2(x-y)d\Delta t F(y) + d^2 \Delta t^2 F(y)^2}{4d\Delta t} \right)\\
& \ \ \  \times \exp \left( \frac{(y-x)^2-2(y-x)d\Delta t F(x) + d^2 \Delta t^2 F(x)^2}{4d\Delta t} \right) \frac{| \Psi_T(y) | ^2}{ | \Psi_T(x) | ^2}\\
&= \exp \left( \frac{2(x-y)d\Delta t (F(y)+F(x)) + d^2 \Delta t^2 (F(x)^2-F(y)^2)}{4d\Delta t} \right) \frac{| \Psi_T(y) | ^2}{ | \Psi_T(x) | ^2}\\
&= \exp \left( \frac{2(x-y) (F(y)+F(x)) + d \Delta t (F(x)^2-F(y)^2)}{4} \right) \frac{| \Psi_T(y) | ^2}{ | \Psi_T(x) | ^2}\\
&= \exp \left( \frac{1}{2}(x-y) (F(y)+F(x)) + \frac{1}{4} d \Delta t (F(x)^2-F(y)^2) \right) \frac{| \Psi_T(y) | ^2}{ | \Psi_T(x) | ^2}\\
\end{align*}




\end{document}